using counter for freshness

theories/Bigstep.v
@@ -9,97 +9,88 @@ Definition var_set := list var.
 Definition in_var_set (x : var) (s : var_set) : bool :=
   existsb (String.eqb x) s.
 
-Open Scope string_scope.
-Inductive eval_expr : heap -> var_set -> expr -> heap -> expr -> Prop :=
-  | EvalWhnf : forall G L w,
+Inductive eval_expr : nat -> heap -> var_set -> expr -> 
+                      heap -> expr -> nat -> Prop :=
+  | EvalWhnf : forall c G L w,
       whnf w ->
-      eval_expr G L w G w
+      eval_expr c G L w G w c
 
-  | EvalSat : forall G L m e D O w,
+  | EvalSat : forall c c1 c2 G L m e D O w,
       matching_arity m = Some 0 ->
-      eval_matching G L [] m D (MRReturn e) ->
-      eval_expr D L e O w ->
-      eval_expr G L (ELam m) O w
+      eval_matching c G L [] m D (MRReturn e) c1 ->
+      eval_expr c1 D L e O w c2 ->
+      eval_expr c G L (ELam m) O w c2
 
-  | EvalVar : forall G L y e D w,
+  | EvalVar : forall c c' G L y e D w,
       heap_lookup G y = Some e ->
       ~ (In y L) ->
-      eval_expr (heap_remove G y) (y :: L) e D w -> (* black-holing *)
-      eval_expr G L (EVar y) (heap_update D y w) w
+      eval_expr c (heap_remove G y) (y :: L) e D w c' -> (* black-holing *)
+      eval_expr c G L (EVar y) (heap_update D y w) w c'
 
-  | EvalApp : forall G L e1 e2 m D O w x,
-      eval_expr G L e1 D (ELam m) ->
-      (* e2 should be a variable *)
+  | EvalApp : forall c c1 c2 G L e1 e2 m D O w x,
+      eval_expr c G L e1 D (ELam m) c1 ->
       e2 = EVar x ->
-      eval_expr D L (ELam (MSupply (EVar x) m)) O w ->
-      eval_expr G L (EApp e1 e2) O w
+      (* e2 should be a variable *)
+      eval_expr c1 D L (ELam (MSupply (EVar x) m)) O w c2 ->
+      eval_expr c G L (EApp e1 e2) O w c2
 
-with eval_matching : heap -> var_set -> list var -> matching -> heap -> matching_result -> Prop :=
-  | EvalReturn : forall G L A e,
-      eval_matching G L A (MReturn e) G (MRReturn (apply_args A e))
+with eval_matching : nat -> heap -> var_set -> list var -> matching -> 
+                     heap -> matching_result -> nat -> Prop :=
+  | EvalReturn : forall c G L A e,
+      eval_matching c G L A (MReturn e) G (MRReturn (apply_args A e)) c
 
-  | EvalMatchFail : forall G L,
-      eval_matching G L [] MFail G MRFail 
-      (* in the paper, the value of A is not restricted in the BSS, but the SSS restricts it to [] *)
+  | EvalMatchFail : forall c G L,
+      eval_matching c G L [] MFail G MRFail c
 
-  | EvalArg : forall G L A x m D u,
-      eval_matching G L (x :: A) m D u ->
-      eval_matching G L A (MSupply (EVar x) m) D u
+  | EvalArg : forall c c' G L A x m D u,
+      eval_matching c G L (x :: A) m D u c' ->
+      eval_matching c G L A (MSupply (EVar x) m) D u c'
 
-  | EvalBindVar : forall G L A x y m D u,
-      eval_matching G L A (subst_matching m y x) D u ->
-      eval_matching G L (y :: A) (MMatch (PVar x) m) D u
+  | EvalBindVar : forall c c' G L A x y m D u,
+      eval_matching c G L A (subst_matching m y x) D u c' ->
+      eval_matching c G L (y :: A) (MMatch (PVar x) m) D u c'
 
-  | EvalConsMatch : forall G L A x c ps m args D O u,
-      eval_expr G L (EVar x) D (ECons c (map EVar args)) ->
+  | EvalConsMatch : forall c c1 c2 G L A x cp ps m args D O u,
+      eval_expr c G L (EVar x) D (ECons cp (map EVar args)) c1 ->
       length ps = length args ->
-      eval_matching D L A (build_nested_matches args ps m) O u ->
-      eval_matching G L (x :: A) (MMatch (PCons c ps) m) O u
+      eval_matching c1 D L A (build_nested_matches args ps m) O u c2 ->
+      eval_matching c G L (x :: A) (MMatch (PCons cp ps) m) O u c2
 
-  | EvalConsFail : forall G L A x c c' ps m args D,
-      eval_expr G L (EVar x) D (ECons c' args) ->
-      c <> c' ->
-      eval_matching G L (x :: A) (MMatch (PCons c ps) m) D MRFail
+  | EvalConsFail : forall c c' G L A x cp cp' ps m args D,
+      eval_expr c G L (EVar x) D (ECons cp' args) c' ->
+      cp <> cp' ->
+      eval_matching c G L (x :: A) (MMatch (PCons cp ps) m) D MRFail c'
 
-  | EvalAltLeft : forall G L A m1 m2 e D,
-      eval_matching G L A m1 D (MRReturn e) ->
-      eval_matching G L A (MAlt m1 m2) D (MRReturn e)
+  | EvalAltLeft : forall c c' G L A m1 m2 e D,
+      eval_matching c G L A m1 D (MRReturn e) c' ->
+      eval_matching c G L A (MAlt m1 m2) D (MRReturn e) c'
 
-  | EvalAltRight : forall G L A m1 m2 D O u,
-      eval_matching G L A m1 D MRFail ->
-      eval_matching D L A m2 O u ->
-      eval_matching G L A (MAlt m1 m2) O u
+  | EvalAltRight : forall c c1 c2 G L A m1 m2 D O u,
+      eval_matching c G L A m1 D MRFail c1 ->
+      eval_matching c1 D L A m2 O u c2 ->
+      eval_matching c G L A (MAlt m1 m2) O u c2
 
-  (* this would require a full alpha equivalence relation *)
-  (*| EvalWhere : forall G L A m binds D u ys renamed_binds renamed_m,*)
-  (*    length ys = length binds ->*)
-  (*    (* ys are fresh w.r.t. G, L, A, m, and bindings *)*)
-  (*    (forall y, In y ys -> ~In y L /\ heap_lookup G y = None) ->*)
-  (*    (* perform renaming *)*)
-  (*    renamed_binds = rename_bindings binds ys ->*)
-  (*    renamed_m = rename_matching m ys binds ->*)
-  (*    (* allocate renamed bindings in heap *)*)
-  (*    eval_matching (allocate_bindings G renamed_binds) L A renamed_m D u ->*)
-  (*    eval_matching G L A (MWhere m binds) D u*)
-
-  (* for now, canonical naming is enough *)
-  | EvalWhere : forall G L A m binds D u,
-    let avoid := List.app L (map fst (StringMap.elements G)) in
-    let ys := generate_fresh_vars "y" (length binds) avoid in
-    eval_matching (allocate_bindings G (rename_bindings binds ys)) L A 
-                  (rename_matching m ys binds) D u ->
-    eval_matching G L A (MWhere m binds) D u
+  | EvalWhere : forall c G L A m binds D u ys renamed_binds renamed_m,
+      (* generate fresh variables using counter *)
+      ys = gen_n_fresh c (length binds) ->
+      (* perform renaming *)
+      renamed_binds = rename_bindings binds ys ->
+      renamed_m = rename_matching m ys binds ->
+      (* allocate renamed bindings and continue with incremented counter *)
+      eval_matching (c + length binds) (allocate_bindings G renamed_binds) L A renamed_m D u (c + length binds) ->
+      eval_matching c G L A (MWhere m binds) D u (c + length binds)
 .
 
-Close Scope string_scope.
 
 Scheme eval_expr_ind_mutual := Induction for eval_expr Sort Prop
 with eval_matching_ind_mutual := Induction for eval_matching Sort Prop.
 
 Combined Scheme eval_ind from eval_expr_ind_mutual, eval_matching_ind_mutual.
 
-Lemma whnf_self_eval : forall G L e,
-  whnf e -> eval_expr G L e G e.
+  
+
+Lemma whnf_self_eval : forall c G L e,
+  whnf e -> eval_expr c G L e G e c.
 Proof.
   intros. constructor. assumption.
 Qed.
@@ -114,8 +105,8 @@ Proof.
   + rewrite IHm1, IHm2. trivial.
 Qed.
 
-Lemma eval_expr_produces_whnf : forall G L e D w,
-  eval_expr G L e D w -> whnf w.
+Lemma eval_expr_produces_whnf : forall c G L e D w c',
+  eval_expr c G L e D w c' -> whnf w.
 Proof.
   intros. induction H; assumption.
 Qed.
@@ -136,30 +127,36 @@ Qed.
 
 Ltac solve_determinism_expr expr_det :=
   match goal with
-  | [ H1 : eval_expr ?G ?L ?e ?D1 ?w1,
-      H2 : eval_expr ?G ?L ?e ?D2 ?w2 |- _ ] =>
-      assert (D1 = D2 /\ w1 = w2) as [?HeqD ?Heqe] by (eapply expr_det; eauto);
+  | [ H1 : eval_expr ?c ?G ?L ?e ?D1 ?w1 ?c1,
+      H2 : eval_expr ?c ?G ?L ?e ?D2 ?w2 ?c2 |- _ ] =>
+      let HeqD := fresh "HeqD" in
+      let Heqe := fresh "Heqe" in
+      let Heqc := fresh "Heqc" in
+      assert (D1 = D2 /\ w1 = w2 /\ c1 = c2) as [HeqD [Heqe Heqc]] by (eapply expr_det; eauto);
       try discriminate; try congruence; subst
   end.
 
 Ltac solve_determinism_match match_det :=
   match goal with
-  | [ H1 : eval_matching ?G ?L ?A ?m ?D1 ?u1,
-      H2 : eval_matching ?G ?L ?A ?m ?D2 ?u2 |- _ ] =>
-      assert (D1 = D2 /\ u1 = u2) as [?HeqD ?Hequ] by (eapply match_det; eauto);
+  | [ H1 : eval_matching ?c ?G ?L ?A ?m ?D1 ?u1 ?c1,
+      H2 : eval_matching ?c ?G ?L ?A ?m ?D2 ?u2 ?c2 |- _ ] =>
+      let HeqD := fresh "HeqD" in
+      let Hequ := fresh "Hequ" in
+      let Heqc := fresh "Heqc" in
+      assert (D1 = D2 /\ u1 = u2 /\ c1 = c2) as [HeqD [Hequ Heqc]] by (eapply match_det; eauto);
       try discriminate; try congruence; subst
   end.
 
-Lemma eval_expr_deterministic : forall G L e D1 w1 D2 w2,
-  eval_expr G L e D1 w1 ->
-  eval_expr G L e D2 w2 ->
-  D1 = D2 /\ w1 = w2
-with eval_matching_deterministic : forall G L A m D1 u1 D2 u2,
-  eval_matching G L A m D1 u1 ->
-  eval_matching G L A m D2 u2 ->
-  D1 = D2 /\ u1 = u2.
+Lemma eval_expr_deterministic : forall c G L e D1 w1 c2 D2 w2 c3,
+  eval_expr c G L e D1 w1 c2 ->
+  eval_expr c G L e D2 w2 c3 ->
+  D1 = D2 /\ w1 = w2 /\ c2 = c3
+with eval_matching_deterministic : forall c G L A m D1 u1 c2 D2 u2 c3,
+  eval_matching c G L A m D1 u1 c2 ->
+  eval_matching c G L A m D2 u2 c3 ->
+  D1 = D2 /\ u1 = u2 /\ c2 = c3.
 Proof.
-  - intros G L e D1 w1 D2 w2 H1 H2.
+  - intros c G L e D1 w1 c2 D2 w2 c3 H1 H2.
     induction H1; inversion H2; subst; try congruence.
     + auto.
     + inversion H; subst. rewrite H0 in H5. discriminate.
@@ -175,12 +172,12 @@ Proof.
       solve_determinism_expr eval_expr_deterministic.
       subst. auto.
     + inversion H0.
-    + inversion H6; subst.
+    + inversion H7; subst.
       solve_determinism_expr eval_expr_deterministic.
       inversion Heqe; subst.
       apply IHeval_expr2. assumption.
 
-  - intros G L A m D1 u1 D2 u2 H1 H2.
+  - intros c G L A m D1 u1 c2 D2 u2 c3 H1 H2.
     induction H1; inversion H2; subst; try congruence; try auto.
     + solve_determinism_expr eval_expr_deterministic.
       injection Heqe as Heqargs.
@@ -191,7 +188,7 @@ Proof.
         injection Heq. trivial.
     + solve_determinism_expr eval_expr_deterministic.
     + solve_determinism_expr eval_expr_deterministic.
-    + split; [ | trivial]. eapply eval_expr_deterministic; eauto.
+    + split; [|split]; [| trivial |]; eapply eval_expr_deterministic; eauto.
     + solve_determinism_match eval_matching_deterministic.
     + solve_determinism_match eval_matching_deterministic.
     + solve_determinism_match eval_matching_deterministic. subst. auto.
